templates: refactor cdl-refine to use object ranges + FP_Eval based proof

camkes/templates/cdl-refine.thy
@@ -22,41 +22,13 @@ imports
   /*? arch_spec_thy ?*/ (* generated arch spec *)
   /*? cdl_thy ?*/ (* generated CDL spec *)
   "CamkesCdlRefine.Policy_CAMKES_CDL"
+  "CamkesCdlRefine.Eval_CAMKES_CDL"
   "DPolicy.Dpolicy"
   "Lib.FastMap"
+  "Lib.RangeMap"
+  "Lib.FP_Eval"
+  "Lib.TermPatternAntiquote"
 begin
-
-section \<open>Generic policy labelling helpers\<close>
-(* FIXME: MOVE *)
-text \<open>Retrieve all frames and page tables mapped into a page directory.\<close>
-definition mapped_pts_of :: "cdl_heap \<Rightarrow> cdl_cap_map \<Rightarrow> cdl_object_id set"
-  where
-  "mapped_pts_of object_map pd_caps \<equiv>
-      {pt_id. \<exists>pt \<in> ran pd_caps. pt_id \<in> cap_objects pt}"
-
-definition mapped_frames_of :: "cdl_heap \<Rightarrow> cdl_cap_map \<Rightarrow> cdl_object_id set"
-  where
-  "mapped_frames_of object_map pd_caps \<equiv>
-      {frame_id.
-         \<exists>pt_id \<in> mapped_pts_of object_map pd_caps.
-           \<exists>frame \<in> ran (object_slots (the (object_map pt_id))).
-             frame_id \<in> cap_objects frame}"
-
-text \<open>
-  Resolve a schematic equality "{a, b, c, ...} = ?val", while checking
-  that the LHS is a concrete set builder expression
-\<close>
-method assign_schematic_set =
-  ((rule arg_cong[where f="insert _"])+, rule refl[where t="{}"])
-
-text \<open>
-  Resolve a schematic equality "(a = x \<and> b = y \<and> c = z \<and> \<dots>) = ?val",
-  while checking that the LHS is a conjunction of equations
-\<close>
-method assign_schematic_eq_conjs =
-  ((rule conj_cong[where P="_ = _", OF refl])+, rule refl[where t="_ = _"])
-
-
 
 section \<open>System-specific policy definitions\<close>
 text \<open>
@@ -64,162 +36,41 @@ text \<open>
   and also allows the cap layout to satisfy the access policy.
 \<close>
 
-ML \<open>
-(* The FastMap package expects the input in sorted order,
-   we need to sort the object IDs by numeric value. *)
-fun /*? options.verification_base_name ?*/_id_value ctxt obj_name =
-    Proof_Context.get_thm ctxt ("/*? cdl_thy ?*/." ^ obj_name ^ "_id_def")
-    |> Thm.prop_of
-    |> Logic.dest_equals |> snd
-    |> HOLogic.dest_number |> snd;
-
-val /*? options.verification_base_name ?*/_obj_labels =
-  sort (apply2 (fst #> /*? options.verification_base_name ?*/_id_value @{context}) #> int_ord)
-    /*- for not_first, (obj, label) in enumerate(sorted(object_label_mapping(), key=lambda('x: x[0].name'))) -*/
-      /*? ',' if not_first else '[' ?*/ ("/*? obj.name ?*/", "/*? label ?*/")
-    /*- endfor -*/
-    ];
-\<close>
-
-local_setup \<open>
-  let
-    val mapping = /*? options.verification_base_name ?*/_obj_labels
-       |> map (fn (obj, label) => (Const ("/*? cdl_thy ?*/." ^ obj ^ "_id", @{typ cdl_object_id}),
-                                   HOLogic.mk_string label));
-    val key_getter = @{term "id :: word32 \<Rightarrow> word32"};
-    val extra_simps = @{thms /*? cdl_thy ?*/.ids};
-  in
-    FastMap.define_map
-      (FastMap.name_opts_default "/*? options.verification_base_name ?*/_labelling")
-      mapping
-      key_getter
-      extra_simps
-      false
-  end
-\<close>
-print_theorems
-
-definition /*? options.verification_base_name ?*/_admissible_labelling :: "label agent_map \<Rightarrow> bool"
-  where
-  "/*? options.verification_base_name ?*/_admissible_labelling label_of \<equiv>
-      (\<forall>i l. /*? options.verification_base_name ?*/_labelling i = Some l \<longrightarrow> label_of i = l)"
-
-lemma /*? options.verification_base_name ?*/_admissible_labelling_default:
-  "/*? options.verification_base_name ?*/_admissible_labelling (the o /*? options.verification_base_name ?*/_labelling)"
-  by (simp add: /*? options.verification_base_name ?*/_admissible_labelling_def)
-
-text \<open>Make sure that an admissible labelling exists.\<close>
-corollary /*? options.verification_base_name ?*/_admissible_labelling_exists:
-  "\<exists>label_of. /*? options.verification_base_name ?*/_admissible_labelling label_of"
-  by (blast intro: /*? options.verification_base_name ?*/_admissible_labelling_default)
-
-text \<open>
-  Helper to unfold the list of object-to-label mappings.
-  The conclusion of admissible_labelling_values will be a conjunction of
-  equations for the label_of function.
-\<close>
-lemma iterate_labelling_helper:
-  "\<lbrakk> /*? options.verification_base_name ?*/_admissible_labelling label_of;
-     /*? options.verification_base_name ?*/_labelling = map_of binds;
-     distinct (map fst binds)
-   \<rbrakk> \<Longrightarrow> list_all (\<lambda>(k, v). label_of k = v) binds"
-  unfolding /*? options.verification_base_name ?*/_admissible_labelling_def
-  by (blast intro: list_allI FastMap.map_of_lookups)
-
-lemmas admissible_labelling_values =
-  iterate_labelling_helper[
-    OF _ /*? options.verification_base_name ?*/_labelling_to_lookup_list /*? options.verification_base_name ?*/_labelling_keys_distinct,
-    simplified FastMap.list_all_dest prod.case]
-
-subsection \<open>Sanity checks for object labelling\<close>
-
-text \<open>
-  Check that we always label certain important objects with the obvious
-  component name. We check this for each component's:
-
-  \begin{itemize}
-    \item Control TCB
-    \item Root CNode (CAmkES only generates one CNode level for each component,
-          so this suffices for now)
-    \item PD and its PTs
-    \item TCB root caps (this also covers the CNode and PD, but includes
-          additional things like the IPC buffer frame)
-  \end{itemize}
-\<close>
-lemma /*? options.verification_base_name ?*/_admissible_labelling__tcbs_correct:
-  "/*? options.verification_base_name ?*/_admissible_labelling label_of \<Longrightarrow>
-      (
-/*- for not_first, c in enumerate(me.composition.instances) -*/
-      /*? '\\<and>' if not_first else ' ' ?*/ label_of /*? c.name ?*/_cnode_id = ''/*? c.name ?*/''
-      \<and> label_of /*? '%s_%d' % (c.name, len(c.name)) ?*/_0_control_9_tcb_id = ''/*? c.name ?*/''
-      \<and> label_of /*? c.name ?*/_group_bin_pd_id = ''/*? c.name ?*/''
-      \<and> (\<forall>cap \<in> ran /*? '%s_%d' % (c.name, len(c.name)) ?*/_0_control_9_tcb_caps. \<forall>i \<in> cap_objects cap. label_of i = ''/*? c.name ?*/'')
-      \<and> (\<forall>pt_i \<in> mapped_pts_of /*? cdl_thy ?*/.objects /*? c.name ?*/_group_bin_pd_caps. label_of pt_i = ''/*? c.name ?*/'')
-/*- endfor -*/
-      )"
-  apply (drule admissible_labelling_values)
-  apply (clarsimp simp: mapped_pts_of_def object_slots_def
-                        /*? cdl_thy ?*/.cap_defs /*? cdl_thy ?*/.obj_defs /*? cdl_thy ?*/.objects)
-  done
-
-text \<open>
-  Also check that all labels are inhabited.
-\<close>
-lemma /*? options.verification_base_name ?*/_admissible_labelling__all_labels_inhabited:
-  "/*? options.verification_base_name ?*/_admissible_labelling label_of \<Longrightarrow>
-/*- for not_first, c in enumerate(me.composition.instances + me.composition.connections) -*/
-     /*? '\\<and>' if not_first else ' ' ?*/ (\<exists>obj. label_of obj = ''/*? c.name ?*/'')
-/*- endfor -*/
-  "
-  apply (drule admissible_labelling_values)
-  apply (elim conjE)
-  apply (intro conjI; erule exI)
-  done
-
-(* FIXME: more sanity checks *)
-
-
-section \<open>More helpers\<close>
+section \<open>Expand policy rules\<close>
 
 definition /*? options.verification_base_name ?*/_policy
   where
   "/*? options.verification_base_name ?*/_policy \<equiv> policy_of /*? arch_spec_thy ?*/.assembly'"
 
+/*# FIXME: naming scheme duplicated from arch-definitions #*/
+/*- if hasattr(me, 'name') and me.name is not none -*/
+    /*- set assembly_name = me.name -*/
+/*- else -*/
+    /*- set assembly_name = 'assembly\'' -*/
+/*- endif -*/
+/*- if hasattr(me.composition, 'name') and me.composition.name is not none -*/
+    /*- set composition_name = me.composition.name -*/
+/*- else -*/
+    /*- set composition_name = 'composition\'' -*/
+/*- endif -*/
 
 schematic_goal /*? options.verification_base_name ?*/_component_names:
   "components (composition /*? arch_spec_thy ?*/.assembly') = ?comps"
-  apply (clarsimp simp: /*? arch_spec_thy ?*/.assembly'_def
-                        /*? arch_spec_thy ?*/.composition'_def)
+  apply (clarsimp simp: /*? arch_spec_thy ?*/./*? assembly_name ?*/_def
+                        /*? arch_spec_thy ?*/./*? composition_name ?*/_def)
   apply (rule refl)
   done
 
 schematic_goal /*? options.verification_base_name ?*/_connections:
   "connections (composition /*? arch_spec_thy ?*/.assembly') = ?spec"
-  apply (clarsimp simp: /*? arch_spec_thy ?*/.assembly'_def
-                        /*? arch_spec_thy ?*/.composition'_def
+  apply (clarsimp simp: /*? arch_spec_thy ?*/./*? assembly_name ?*/_def
+                        /*? arch_spec_thy ?*/./*? composition_name ?*/_def
 /*- for c in me.composition.instances + me.composition.connections -*/
                         /*? arch_spec_thy ?*/./*? c.name ?*/_def
 /*- endfor -*/
         )
   apply (rule refl)
   done
-
-text \<open>
-  Resolve a schematic equality of the form
-  "((a1 = x1 \<and> a2 = x2 \<and> \<dots>) \<or> (b1 = y1 \<and> b2 = y2 \<and> \<dots>) \<or> \<dots>) = ?val",
-  while ensuring that the LHS consists of equations in disjunctive normal form.
-\<close>
-method assign_schematic_dnf =
-  ((rule disj_cong, assign_schematic_eq_conjs)+, assign_schematic_eq_conjs)
-
-lemma split_Collect_graph_edge:
-  "Collect P = Collect (\<lambda>(from, auth, to). P (from, auth, to))"
-  by simp
-
-lemma Collect_graph_cong_helper:
-  "(\<And>x y z. P x y z = P' x y z) \<Longrightarrow>
-   Collect (\<lambda>(x, y, z). P x y z) = Collect (\<lambda>(x, y, z). P' x y z)"
-  by simp
 
 schematic_goal /*? options.verification_base_name ?*/_policy_def':
   "/*? options.verification_base_name ?*/_policy = ?PAS"
@@ -268,6 +119,148 @@ local_setup {* fn ctxt => let
 *}
 thm /*? options.verification_base_name ?*/_policy_intros
 
+
+section \<open>Object label mappings\<close>
+
+text \<open>
+  Construct mapping of integrity labels for each object.
+\<close>
+
+ML \<open>
+(* The RangeMap package expects the input in sorted order,
+   we need to sort the object IDs by numeric value. *)
+fun /*? options.verification_base_name ?*/_id_value ctxt obj_name =
+    Proof_Context.get_thm ctxt ("/*? cdl_thy ?*/." ^ obj_name ^ "_id_def")
+    |> Thm.prop_of
+    |> Logic.dest_equals |> snd
+    |> HOLogic.dest_number |> snd;
+
+val /*? options.verification_base_name ?*/_obj_labels =
+  sort (apply2 (#1 #> /*? options.verification_base_name ?*/_id_value @{context}) #> int_ord)
+      (* object name, size bits, policy label *)
+    /*- set delim = namespace(value='[') -*//*# need this nonsense to modify variable -- see jinja2 docs #*/
+    /*- for (obj, label) in sorted(object_label_mapping(), key=lambda('x: x[0].name')) -*/
+      /*- if not obj.name.startswith('root_untyped_') -*//*# Exclude root untypeds because they overlap other objects and have no policy. FIXME: better way to detect these #*/
+        /*? delim.value ?*/ ("/*? obj.name ?*/", /*? obj.get_size_bits() ?*/, "/*? label ?*/")
+        /*- set delim.value = ',' -*/
+      /*- endif -*/
+    /*- endfor -*/
+    ];
+
+val id_value : string -> int =
+  fn id =>
+    Proof_Context.get_thm @{context} (id ^ "_def")
+    |> Thm.rhs_of |> Thm.term_of |> HOLogic.dest_number |> snd;
+
+(* Now construct our mapping from (ptr, ptr + 2^sz) to labels *)
+val /*? options.verification_base_name ?*/_label_entries =
+  /*? options.verification_base_name ?*/_obj_labels
+  |> map (fn (obj_name, sz, label) => ("/*? cdl_thy ?*/." ^ obj_name ^ "_id", sz, label))
+  |> map (fn (id, sz, label) =>
+            ((Const (id, @{typ cdl_object_id}),
+              @{term "(+) :: cdl_object_id \<Rightarrow> _ \<Rightarrow> _"} $
+                Const (id, @{typ cdl_object_id}) $
+                (@{term "(^) 2 :: _ \<Rightarrow> cdl_object_id"} $ HOLogic.mk_number @{typ nat} sz)),
+             HOLogic.mk_string label))
+  |> map (fn (range, label) =>
+      (apply2 (Thm.cterm_of @{context}) range, Thm.cterm_of @{context} label));
+\<close>
+
+local_setup \<open>
+  RangeMap.define_map (RangeMap.name_opts_default "/*? options.verification_base_name ?*/_label")
+      /*? options.verification_base_name ?*/_label_entries @{typ cdl_object_id} @{typ label}
+      (FP_Eval.eval_conv @{context}
+        (FP_Eval.make_rules @{thms word_rel_simps_small word_pow_arith_simps /*? cdl_thy ?*/.ids} []))
+\<close>
+(* we will primarily use these *)
+lemmas /*? options.verification_base_name ?*/_label_lookups =
+  /*? options.verification_base_name ?*/_label.start_lookups
+    [unfolded /*? options.verification_base_name ?*/_label.tree_list_lookup_eq]
+
+text \<open>
+  Define admissible labelling functions to be those that are consistent
+  with the mapping we defined above.
+\<close>
+
+definition /*? options.verification_base_name ?*/_labelling :: "cdl_object_id \<Rightarrow> string option"
+  where
+  "/*? options.verification_base_name ?*/_labelling x \<equiv> map_option snd (RangeMap.range_map_of /*? options.verification_base_name ?*/_label.list x)"
+
+definition /*? options.verification_base_name ?*/_admissible_labelling :: "label agent_map \<Rightarrow> bool"
+  where
+  "/*? options.verification_base_name ?*/_admissible_labelling label_of \<equiv>
+      (\<forall>i l. /*? options.verification_base_name ?*/_labelling i = Some l \<longrightarrow> label_of i = l)"
+
+lemma /*? options.verification_base_name ?*/_admissible_labelling_default:
+  "/*? options.verification_base_name ?*/_admissible_labelling (the o /*? options.verification_base_name ?*/_labelling)"
+  by (simp add: /*? options.verification_base_name ?*/_admissible_labelling_def)
+
+text \<open>Make sure that an admissible labelling exists.\<close>
+corollary /*? options.verification_base_name ?*/_admissible_labelling_exists:
+  "\<exists>label_of. /*? options.verification_base_name ?*/_admissible_labelling label_of"
+  by (blast intro: /*? options.verification_base_name ?*/_admissible_labelling_default)
+
+
+subsection \<open>Sanity checks for object labelling\<close>
+
+text \<open>
+  Check that we always label certain important objects with the obvious
+  component name. We check this for each component's:
+
+  \begin{itemize}
+    \item Control TCB
+    \item Root CNode (CAmkES only generates one CNode level for each component,
+          so this suffices for now)
+    \item PD and its PTs
+    \item TCB root caps (this also covers the CNode and PD, but includes
+          additional things like the IPC buffer frame)
+  \end{itemize}
+\<close>
+lemma /*? options.verification_base_name ?*/_admissible_labelling__tcbs_correct:
+  "/*? options.verification_base_name ?*/_admissible_labelling label_of \<Longrightarrow>
+      (
+/*- for not_first, c in enumerate(me.composition.instances) -*/
+      /*? '\\<and>' if not_first else ' ' ?*/ label_of /*? c.name ?*/_cnode_id = ''/*? c.name ?*/''
+      \<and> label_of /*? '%s_%s' % (c.name, c.name) ?*/_0_control_tcb_id = ''/*? c.name ?*/''
+      \<and> label_of /*? c.name ?*/_group_bin_pd_id = ''/*? c.name ?*/''
+      \<and> (\<forall>cap \<in> ran /*? '%s_%s' % (c.name, c.name) ?*/_0_control_tcb_caps. \<forall>i \<in> cap_objects cap. label_of i = ''/*? c.name ?*/'')
+      \<and> (\<forall>pt_i \<in> mapped_pts_of /*? cdl_thy ?*/.objects /*? c.name ?*/_group_bin_pd_caps. label_of pt_i = ''/*? c.name ?*/'')
+/*- endfor -*/
+      )"
+  (* FIXME: cleanup *)
+  apply (simp only: rel_simps arith_simps simp_thms if_False if_True conj_assoc imp_disjL
+                    option.map prod.sel
+                    ball_simps bex_simps fun_upd_apply ran_map_upd ran_empty
+                    finite_set_simps
+                    cdl_cap.case cap_objects.simps mapped_pts_of_def object_slots_def
+
+                    /*? options.verification_base_name ?*/_CDL.cap_defs
+                    /*? options.verification_base_name ?*/_CDL.obj_defs
+                    /*? options.verification_base_name ?*/_CDL.objects_lookups
+
+                    /*? options.verification_base_name ?*/_admissible_labelling_def
+                    /*? options.verification_base_name ?*/_labelling_def
+                    /*? options.verification_base_name ?*/_label_lookups
+              cong: imp_cong)
+  done
+
+text \<open>
+  Also check that all labels are inhabited.
+\<close>
+lemma /*? options.verification_base_name ?*/_admissible_labelling__all_labels_inhabited:
+  "/*? options.verification_base_name ?*/_admissible_labelling label_of \<Longrightarrow>
+/*- for not_first, c in enumerate(me.composition.instances + me.composition.connections) -*/
+     /*? '\\<and>' if not_first else ' ' ?*/ (\<exists>obj. label_of obj = ''/*? c.name ?*/'')
+/*- endfor -*/
+  "
+  apply (simp add: /*? options.verification_base_name ?*/_admissible_labelling_def
+                   /*? options.verification_base_name ?*/_labelling_def)
+  apply (fastforce intro: /*? options.verification_base_name ?*/_label_lookups)
+  done
+
+(* FIXME: more sanity checks *)
+
+
 section \<open>Admissible PAS\<close>
 
 text \<open>
@@ -297,32 +290,6 @@ lemma /*? options.verification_base_name ?*/_admissible_pas_exists:
   done
 
 text \<open>
-  Simplified, automation-friendl(ier) intro for policy_wellformed, assuming that
-  CAmkES never provides Grant auth across components and IRQs are disabled.
-\<close>
-
-lemma camkes_policy_wellformedI:
-  assumes "\<not>maySendIrqs"
-      and "\<And>a. (agent, a, agent) \<in> aag"
-      and "\<And>s auth r. (s, auth, r) \<in> aag \<Longrightarrow> (s, Control, s) \<in> aag"
-      and "\<And>s r. (s, Grant, r) \<in> aag \<Longrightarrow> s = r"
-      and "\<And>s r. (s, Control, r) \<in> aag \<Longrightarrow> s = r"
-      and "\<And>s auth. (s, Control, s) \<in> aag \<Longrightarrow> (s, auth, s) \<in> aag"
-      and "\<And>s r. (s, Receive, r) \<in> aag \<Longrightarrow> s \<noteq> r \<Longrightarrow> (r, Control, r) \<in> aag \<Longrightarrow> False"
-      and "\<And>s r. (s, Call, r) \<in> aag \<Longrightarrow> s \<noteq> r \<Longrightarrow> (r, Control, r) \<in> aag \<Longrightarrow> False"
-      and "\<And>s ep. (s, Call, ep) \<in> aag \<Longrightarrow> (s, SyncSend, ep) \<in> aag"
-      and "\<And>s r. (s, Reply, r) \<in> aag \<Longrightarrow> (r, DeleteDerived, s) \<in> aag"
-      and "\<And>s r ep. (s, Call, ep) \<in> aag \<Longrightarrow> s \<noteq> ep \<Longrightarrow> (r, Receive, ep) \<in> aag
-                     \<Longrightarrow> (r, Reply, s) \<in> aag"
-      and "\<And>l1 l2 l3. (l1, DeleteDerived, l2) \<in> aag \<Longrightarrow> l1 \<noteq> l2 \<Longrightarrow> (l2, DeleteDerived, l3) \<in> aag
-                       \<Longrightarrow> (l1, DeleteDerived, l3) \<in> aag"
-  shows "policy_wellformed aag maySendIrqs irqSet agent"
-  unfolding policy_wellformed_def
-  apply (insert assms)
-  apply (safe; metis)
-  done
-
-text \<open>
   Checking the transitivity conditions for @{const policy_wellformed} is quadratic in
   the size of our policy; here we extract relevant subsets of the policy cases to
   make things a bit faster.
@@ -339,7 +306,7 @@ lemmas /*? options.verification_base_name ?*/_policy_cases_Receive =
 lemmas /*? options.verification_base_name ?*/_policy_cases_Reply =
   /*? options.verification_base_name ?*/_policy_gen_cases_[where auth = "Reply", simplified]
 lemmas /*? options.verification_base_name ?*/_policy_cases_Grant =
-  /*? options.verification_base_name ?*/_policy_gen_cases_[where auth = "Grant", simplified]
+  /*? options.verification_base_name ?*/_policy_gen_cases_[where auth = "auth.Grant", simplified]
 lemmas /*? options.verification_base_name ?*/_policy_cases_Call =
   /*? options.verification_base_name ?*/_policy_gen_cases_[where auth = "Call", simplified]
 lemmas /*? options.verification_base_name ?*/_policy_cases_DeleteDerived =
@@ -405,218 +372,203 @@ lemma /*? options.verification_base_name ?*/_policy_wellformed:
          simp only: /*? options.verification_base_name ?*/_policy_intros)
   done
 
-section \<open>More helpers\<close>
-
-(* FIXME: Gap in the Dpolicy model, object ID semantic mismatch between ASpec and DSpec (VER-924) *)
-lemma cdl_obj_refs_frame_cheat:
-  "cdl_obj_refs (cdl_cap.FrameCap dev x rs sz is_real asid) = {x}"
-  sorry
-declare cdl_obj_refs.simps(16)[simp del]
-declare cdl_obj_refs_frame_cheat[simp]
-
-lemmas cdl_obj_refs_cheat_simps =
-  cdl_obj_refs.simps(1-15) cdl_obj_refs_frame_cheat cdl_obj_refs.simps(17-)
-
-lemma iterate_add_map_helper:
-  (* m0 will be empty_irq_objects *)
-  "\<lbrakk> (m0 ++ m(k \<mapsto> v)) a = Some b;
-     \<lbrakk> a = k; b = v \<rbrakk> \<Longrightarrow> P;
-     \<lbrakk> (m0 ++ m) a = Some b \<rbrakk> \<Longrightarrow> P
-   \<rbrakk> \<Longrightarrow> P"
-  (* \<open>simp split: if_split\<close> loops *)
-  apply simp
-  apply (subst (asm) if_split[where P="\<lambda>x. x = _"])
-  apply fastforce
-  done
-
-lemma iterate_map_helper:
-  "\<lbrakk> (m(k \<mapsto> v)) a = Some b;
-     \<lbrakk> a = k; b = v \<rbrakk> \<Longrightarrow> P;
-     \<lbrakk> m a = Some b \<rbrakk> \<Longrightarrow> P
-   \<rbrakk> \<Longrightarrow> P"
-  using iterate_add_map_helper[where m0=Map.empty]
-  by fastforce
-
-lemma case_obj_helper:
-  "\<lbrakk> (case (m0 ++ m(k \<mapsto> v)) a of None \<Rightarrow> n | Some y \<Rightarrow> s y) b = Some cap;
-     \<lbrakk> a = k; s v b = Some cap \<rbrakk> \<Longrightarrow> P;
-     \<lbrakk> (case (m0 ++ m) a of None \<Rightarrow> n | Some y \<Rightarrow> s y) b = Some cap \<rbrakk> \<Longrightarrow> P
-   \<rbrakk> \<Longrightarrow> P"
-  by (simp split: if_splits)
-
-lemmas object_slots_eval_simps =
-    object_slots_def cdl_object.case
-    cdl_asid_pool.simps
-    cdl_cnode.simps
-    cdl_irq_node.simps
-    cdl_page_table.simps
-    cdl_page_directory.simps
-    cdl_tcb.simps
-
 
 
 section \<open>CAmkES-capDL refinement proof\<close>
 
-text \<open>Helpers to put the policy subgoals into a consistent form for our automation\<close>
-lemma helper_pcs_refined_policyI:
-  assumes cdt_policy: "\<And>p slot p' slot'.
-                          cdl_cdt s (p, slot) = Some (p', slot') \<Longrightarrow>
-                          (pasObjectAbs aag p', Control, pasObjectAbs aag p) \<in> pasPolicy aag"
-      and delete_derived_policy: "\<And>p slot p' slot'.
-                          cdl_cdt s (p, slot) = Some (p', slot') \<Longrightarrow>
-                          (pasObjectAbs aag p', DeleteDerived, pasObjectAbs aag p) \<in> pasPolicy aag"
-      and obj_policy: "\<And>p p_obj p_idx cap auth oref.
-                          \<lbrakk> cdl_objects s p = Some p_obj;
-                            object_slots p_obj p_idx = Some cap;
-                            auth \<in> cdl_cap_auth_conferred cap;
-                            oref \<in> cdl_obj_refs cap
-                          \<rbrakk> \<Longrightarrow> (pasObjectAbs aag p, auth, pasObjectAbs aag oref) \<in> pasPolicy aag"
-  shows "auth_graph_map (pasObjectAbs aag) (cdl_state_objs_to_policy s) \<subseteq> (pasPolicy aag)"
-  apply (clarsimp simp: cdl_state_objs_to_policy_def auth_graph_map_def)
-  by (fastforce elim: cdl_state_bits_to_policy.cases
-                intro: obj_policy cdt_policy delete_derived_policy
-                simp: opt_cap_def slots_of_def opt_object_def
-                split: option.splits)
+(* specialise ptr_range rewrite rule *)
+lemmas /*? options.verification_base_name ?*/_label_over_ptr_range =
+  label_over_ptr_range[
+      (* FP_Eval only supports first-order matching, so instantiate P *)
+      where P = "\<lambda>l. (_, _, l) \<in> _" and label_spec = /*? options.verification_base_name ?*/_labelling,
+      OF /*? options.verification_base_name ?*/_label.list_monotonic,
+      (* expand labelling into tree lookup *)
+      unfolded /*? options.verification_base_name ?*/_labelling_def, OF refl]
+lemmas /*? options.verification_base_name ?*/_label_over_ptr_range_cases =
+  /*? options.verification_base_name ?*/_label_lookups[THEN /*? options.verification_base_name ?*/_label_over_ptr_range]
 
 text \<open>FIXME: Our capDL assigns no ASIDs, so there's not much to do here right now.\<close>
 lemma /*? options.verification_base_name ?*/_asid_policy_trivial:
-  "cdl_state_asids_to_policy pas /*? cdl_thy ?*/.state \<subseteq> pasPolicy pas"
-  apply (clarsimp simp: /*? cdl_thy ?*/.state_def /*? cdl_thy ?*/.asid_table_def
-                        opt_cap_def slots_of_def opt_object_def object_slots_def)
-  apply (erule cdl_state_asids_to_policy_aux.cases)
-    (* ASIDs in CDL heap*)
-    (* unfold object map *)
-    apply clarsimp
-    apply (simp only: /*? cdl_thy ?*/.objects_def)
+  assumes admissible_pas:
+     "/*? options.verification_base_name ?*/_admissible_pas pas"
+  shows
+    "cdl_state_asids_to_policy pas /*? options.verification_base_name ?*/_CDL.state \<subseteq> pasPolicy pas"
+proof -
+  (* everything needed to evaluate asid integrity... *)
+  note obj_policy_eval_simps' =
+        /*? options.verification_base_name ?*/_label_lookups
+        /*? options.verification_base_name ?*/_CDL.obj_defs
+        (* Map.empty is actually an abbrev for a lambda, which fp_eval
+           doesn't allow as a rule LHS. Rewrite eagerly first *)
+        (* FIXME: generate these with map_of in the first place.
+           Also fix "rev ..." in graph_of_map_of__sorted_eval *)
+        /*? options.verification_base_name ?*/_CDL.cap_defs[simplified fun_upds_to_map_of]
+        /*? options.verification_base_name ?*/_label_over_ptr_range_cases
 
-    (* traverse mapping *)
-    apply (match premises in
-                "case_option _ _ ((_ ++ _(_ \<mapsto> obj)) _) _ = _" for obj \<Rightarrow> \<open>print_term obj\<close>,
-           erule case_obj_helper,
-           time_methods \<open>solves \<open>simp add: /*? cdl_thy ?*/.obj_defs;
-                                 (simp only: /*? cdl_thy ?*/.cap_defs,
-                                  (erule iterate_map_helper, solves \<open>simp\<close>)+,
-                                  solves \<open>simp\<close>)\<close>\<close>)+
-    apply (solves \<open>clarsimp simp: /*? cdl_thy ?*/.empty_irq_objects_def /*? cdl_thy ?*/.empty_irq_node_def
-                            split: if_split_asm\<close>)
-   (* ASID lookup case *)
-   apply blast
-  (* ASID pool case *)
-  apply blast
-  done
+        obj_policy_eval_simps
+
+  show ?thesis
+    apply (rule cdl_state_asids_to_policy__eval[where
+                  policy_spec=/*? options.verification_base_name ?*/_policy and
+                  obj_label_spec=/*? options.verification_base_name ?*/_labelling and
+                  asid_label_spec="\<lambda>_. None"
+           ])
+        using admissible_pas /*? options.verification_base_name ?*/_admissible_pas_def apply blast
+       using admissible_pas /*? options.verification_base_name ?*/_admissible_pas_def /*? options.verification_base_name ?*/_admissible_labelling_def apply blast
+      apply blast
+
+     (* ASIDs in objects *)
+     apply (simp only: /*? options.verification_base_name ?*/_labelling_def)
+     apply (tactic \<open>let
+              val rules = @{thms /*? options.verification_base_name ?*/_CDL.state_def cdl_state.simps
+                                 /*? options.verification_base_name ?*/_CDL.objects_to_lookup_list
+                                 graph_of_map_of__distinct_eval if_True
+                                 /*? options.verification_base_name ?*/_CDL.objects_keys_distinct};
+              val congs = @{thms obj_policy_eval_congs};
+              in SUBGOAL (fn _ => FP_Eval.eval_tac @{context} (FP_Eval.make_rules rules congs) 1)
+                         1 end\<close>)
+     (* this is a separate step for now, because graph_of_map_of__sorted_eval
+        won't work for objects list *)
+     apply (tactic \<open>let
+              val rules = @{thms obj_policy_eval_simps'};
+              val congs = @{thms obj_policy_eval_congs};
+              val conv = rpair FP_Eval.skel0
+                       #> FP_Eval.eval @{context} (FP_Eval.make_rules rules congs)
+                       #> tap (fn (_, c) => tracing ("fp_eval counters: " ^ @{make_string} c))
+                       #> fst #> fst;
+              in SUBGOAL (fn _ => Conv.gconv_rule conv 1 #> Seq.succeed) 1 end\<close>;
+            intro TrueI conjI /*? options.verification_base_name ?*/_policy_intros)
+
+    (* ASID pools *)
+    apply (simp add: /*? options.verification_base_name ?*/_CDL.state_def /*? options.verification_base_name ?*/_CDL.asid_table_def graph_of_def)
+    done
+qed
 
 text \<open>FIXME: Our capDL assigns no IRQs, so there's not much to do here right now.\<close>
 lemma /*? options.verification_base_name ?*/_irq_policy_trivial:
-  "cdl_state_irqs_to_policy pas /*? cdl_thy ?*/.state \<subseteq> pasPolicy pas"
-  apply clarsimp
-  apply (erule cdl_state_irqs_to_policy_aux.cases)
-  apply (clarsimp simp: /*? cdl_thy ?*/.state_def /*? cdl_thy ?*/.irqs_def
-                        opt_cap_def slots_of_def opt_object_def object_slots_def)
-  (* unfold object map *)
-  apply (simp only: /*? cdl_thy ?*/.objects_def)
+  assumes admissible_pas:
+     "/*? options.verification_base_name ?*/_admissible_pas pas"
+  shows
+    "cdl_state_irqs_to_policy pas /*? options.verification_base_name ?*/_CDL.state \<subseteq> pasPolicy pas"
+proof -
+  (* everything needed to evaluate asid integrity... *)
+  note obj_policy_eval_simps' =
+        /*? options.verification_base_name ?*/_label_lookups
+        /*? options.verification_base_name ?*/_CDL.obj_defs
+        (* Map.empty is actually an abbrev for a lambda, which fp_eval
+           doesn't allow as a rule LHS. Rewrite eagerly first *)
+        (* FIXME: generate these with map_of in the first place.
+           Also fix "rev ..." in graph_of_map_of__sorted_eval *)
+        /*? options.verification_base_name ?*/_CDL.cap_defs[simplified fun_upds_to_map_of]
+        /*? options.verification_base_name ?*/_label_over_ptr_range_cases
 
-  (* traverse mapping *)
-  apply (match premises in
-              "case_option _ _ ((_ ++ _(_ \<mapsto> obj)) _) _ = _" for obj \<Rightarrow> \<open>print_term obj\<close>,
-         erule case_obj_helper,
-         time_methods \<open>solves \<open>simp add: /*? cdl_thy ?*/.obj_defs;
-                               (simp only: /*? cdl_thy ?*/.cap_defs,
-                                (erule iterate_map_helper, solves \<open>simp\<close>)+,
-                                solves \<open>simp\<close>)\<close>\<close>)+
-  apply (solves \<open>clarsimp simp: /*? cdl_thy ?*/.empty_irq_objects_def /*? cdl_thy ?*/.empty_irq_node_def
-                          split: if_split_asm\<close>)
-  done
+        obj_policy_eval_simps
+
+  show ?thesis
+    apply (rule cdl_state_irqs_to_policy__eval[where
+                  policy_spec=/*? options.verification_base_name ?*/_policy and
+                  obj_label_spec=/*? options.verification_base_name ?*/_labelling and
+                  irq_label_spec="\<lambda>_. None"
+           ])
+       using admissible_pas /*? options.verification_base_name ?*/_admissible_pas_def apply blast
+      using admissible_pas /*? options.verification_base_name ?*/_admissible_pas_def /*? options.verification_base_name ?*/_admissible_labelling_def apply blast
+     apply blast
+
+    apply (simp only: /*? options.verification_base_name ?*/_labelling_def)
+    apply (tactic \<open>let
+             val rules = @{thms /*? options.verification_base_name ?*/_CDL.state_def cdl_state.simps
+                                /*? options.verification_base_name ?*/_CDL.objects_to_lookup_list
+                                graph_of_map_of__distinct_eval if_True
+                                /*? options.verification_base_name ?*/_CDL.objects_keys_distinct};
+             val congs = @{thms obj_policy_eval_congs};
+             in SUBGOAL (fn _ => FP_Eval.eval_tac @{context} (FP_Eval.make_rules rules congs) 1)
+                        1 end\<close>)
+    (* this is a separate step for now, because graph_of_map_of__sorted_eval
+       won't work for objects list *)
+    apply (tactic \<open>let
+             val rules = @{thms obj_policy_eval_simps'};
+             val congs = @{thms obj_policy_eval_congs};
+             val conv = rpair FP_Eval.skel0
+                      #> FP_Eval.eval @{context} (FP_Eval.make_rules rules congs)
+                      #> tap (fn (_, c) => tracing ("fp_eval counters: " ^ @{make_string} c))
+                      #> fst #> fst;
+             in SUBGOAL (fn _ => Conv.gconv_rule conv 1 #> Seq.succeed) 1 end\<close>;
+           intro TrueI conjI /*? options.verification_base_name ?*/_policy_intros)
+    done
+qed
 
 text \<open>Main integrity proof\<close>
 
 theorem /*? options.verification_base_name ?*/_pcs_refined:
   assumes other_assms:
      "pas_wellformed pas"
-     (* TODO *) "cdl_irq_map_wellformed pas /*? cdl_thy ?*/.state"
-     (* TODO *) "cdl_tcb_domain_map_wellformed pas /*? cdl_thy ?*/.state"
+     (* TODO *) "cdl_irq_map_wellformed pas /*? options.verification_base_name ?*/_CDL.state"
+     (* TODO *) "cdl_tcb_domain_map_wellformed pas /*? options.verification_base_name ?*/_CDL.state"
   assumes admissible_pas:
      "/*? options.verification_base_name ?*/_admissible_pas pas"
   shows
-     "pcs_refined pas /*? cdl_thy ?*/.state"
+     "pcs_refined pas /*? options.verification_base_name ?*/_CDL.state"
 proof -
   from admissible_pas have /*? options.verification_base_name ?*/_policy:
     "/*? options.verification_base_name ?*/_policy \<subseteq> pasPolicy pas"
     by (simp add: /*? options.verification_base_name ?*/_admissible_pas_def)
 
-  (* HACK to split the labelling values theorem into multiple equations.
-     We put them into the simpset for fast lookup during the proof procedure.
-     This uses the conjuncts attribute from Lib, which stashes the result into
-     the dynamic theorem "conjuncts". We retrieve it from there. *)
-  note dummy = admissible_labelling_values
-            [OF /*? options.verification_base_name ?*/_admissible_pas_def[simplified atomize_eq, THEN iffD1, THEN conjunct1],
-             OF admissible_pas, simplified atomize_conj[symmetric], conjuncts]
-  note labelling_values = conjuncts
-  (* end hack *)
+  (* everything needed to evaluate object integrity... *)
+  note obj_policy_eval_simps' =
+        /*? options.verification_base_name ?*/_label_lookups
+        /*? options.verification_base_name ?*/_CDL.obj_defs
+        (* Map.empty is actually an abbrev for a lambda, which fp_eval
+           doesn't allow as a rule LHS. Rewrite eagerly first *)
+        (* FIXME: generate these with map_of in the first place.
+           Also fix "rev ..." in graph_of_map_of__sorted_eval *)
+        /*? options.verification_base_name ?*/_CDL.cap_defs[simplified fun_upds_to_map_of]
+        /*? options.verification_base_name ?*/_label_over_ptr_range_cases
+
+        obj_policy_eval_simps
 
   show ?thesis
     apply (clarsimp simp only: simp_thms
                                pcs_refined_def other_assms
-                               /*? options.verification_base_name ?*/_asid_policy_trivial /*? options.verification_base_name ?*/_irq_policy_trivial
+                               /*? options.verification_base_name ?*/_asid_policy_trivial[OF admissible_pas]
+                               /*? options.verification_base_name ?*/_irq_policy_trivial[OF admissible_pas]
                     del: subsetI)
-    apply (rule helper_pcs_refined_policyI)
+    apply (rule helper_pcs_refined_policy__eval[
+                  where policy_spec = /*? options.verification_base_name ?*/_policy
+                    and label_spec = /*? options.verification_base_name ?*/_labelling])
+        (* instantiate policy specs *)
+        apply (rule /*? options.verification_base_name ?*/_policy)
+       using admissible_pas /*? options.verification_base_name ?*/_admissible_pas_def /*? options.verification_base_name ?*/_admissible_labelling_def
+       apply blast
+
       text \<open>
          CDT properties.
          FIXME: Our capDL assigns an empty CDT, so there's not much to do here right now.
       \<close>
-      apply ((fastforce simp: /*? cdl_thy ?*/.state_def /*? cdl_thy ?*/.cdt_def)+)[2]
+      apply ((fastforce simp: /*? options.verification_base_name ?*/_CDL.state_def /*? options.verification_base_name ?*/_CDL.cdt_def)+)[2]
 
     text \<open>Object case.\<close>
-    apply (clarsimp simp: /*? cdl_thy ?*/.state_def)
-
-    (* Assume /*? options.verification_base_name ?*/_policy is concrete enough and we don't need any
-       default policy rules from pas_wellformed. *)
-    apply (rule subsetD[OF /*? options.verification_base_name ?*/_policy])
-
-    (* Unfold big object mapping. *)
-    apply (simp only: /*? cdl_thy ?*/.objects_def)
-
-    (* Cache rulesets to speed up the "solve policy" steps slightly *)
-    supply /*? options.verification_base_name ?*/_policy_intros[intro!]
-    supply labelling_values[simp]
-
-    (* Iterate through all objects and their contained caps (if any) *)
-    apply (match premises in
-                "(_ ++ _(_ \<mapsto> obj)) _ = _" for obj \<Rightarrow> \<open>print_term obj\<close>,
-           (* trivial case: objects without caps *)
-           time_methods
-             cap_non_container_tac:
-                 \<open>erule iterate_add_map_helper,
-                  solves \<open>simp only: object_slots_def /*? cdl_thy ?*/.obj_defs
-                                     option.inject option.distinct cdl_object.case\<close>\<close>
-           (* nontrivial case: objects with caps *)
-          |time_methods
-             cap_to_container_tac:
-                 \<open>erule iterate_add_map_helper,
-                  (* Substitute object value and then remove it (to reduce clutter) *)
-                  simp only:,
-                  thin_tac "p_obj = _",
-                  solves \<open>(simp add: /*? cdl_thy ?*/.cap_defs /*? cdl_thy ?*/.obj_defs,
-                           (* Evaluate object_slots, but do not unfold cap maps
-                              inside the objects yet *)
-                           simp only: object_slots_eval_simps);
-                          (time_methods "  contained cap auth":
-                              \<open>match premises in
-                                 "(_(_ \<mapsto> child_cap)) _ = _"
-                                    for child_cap \<Rightarrow> \<open>print_term child_cap\<close>,
-                               erule iterate_map_helper,
-                               time_methods "    solve policy":
-                                 \<open>fastforce simp: cdl_cap_auth_conferred_def
-                                                  cap_rights_to_auth_def
-                                                  vspace_cap_rights_to_auth_def\<close>\<close>)+,
-                           solves \<open>simp only: option.distinct\<close>\<close>\<close>)+
-
-    (* Assert that we have processed all normal objects *)
-    apply (match premises in "(empty_irq_objects ++ Map.empty) _ = Some _" \<Rightarrow> succeed)
-
-    text \<open>FIXME: Our capDL assigns no IRQs, so there's not much to do here right now.\<close>
-    apply (clarsimp simp: /*? cdl_thy ?*/.empty_irq_objects_def /*? cdl_thy ?*/.empty_irq_node_def
-                          object_slots_def
-                    split: if_split_asm)
+    apply (simp only: /*? options.verification_base_name ?*/_labelling_def)
+    (* this is a separate step for now, because graph_of_map_of__sorted_eval
+       won't work for objects list *)
+    apply (tactic \<open>let
+             val rules = @{thms /*? options.verification_base_name ?*/_CDL.state_def cdl_state.simps
+                                /*? options.verification_base_name ?*/_CDL.objects_to_lookup_list
+                                graph_of_map_of__distinct_eval if_True
+                                /*? options.verification_base_name ?*/_CDL.objects_keys_distinct};
+             val congs = @{thms obj_policy_eval_congs};
+             in SUBGOAL (fn _ => FP_Eval.eval_tac @{context} (FP_Eval.make_rules rules congs) 1)
+                        1 end\<close>)
+    (* this is a separate step for now, because graph_of_map_of__sorted_eval
+       won't work for objects list *)
+    apply (tactic \<open>let
+             val rules = @{thms obj_policy_eval_simps'};
+             val congs = @{thms obj_policy_eval_congs};
+             val conv = rpair FP_Eval.skel0
+                      #> FP_Eval.eval @{context} (FP_Eval.make_rules rules congs)
+                      #> tap (fn (_, c) => tracing ("fp_eval counters: " ^ @{make_string} c))
+                      #> fst #> fst;
+             in SUBGOAL (fn _ => Conv.gconv_rule conv 1 #> Seq.succeed) 1 end\<close>;
+           intro TrueI conjI /*? options.verification_base_name ?*/_policy_intros)
     done
 qed
 
